src/lowparse/LowParse.SLow.DER.fst
@@ -67,55 +67,6 @@ let parse32_der_length_payload32
           else Some ((y <: refine_with_tag tag_of_der_length32 x), consumed)
   ) <: (res: _ { parser32_correct (parse_der_length_payload32 x) input res } ))
 
-inline_for_extraction
-let der_length_payload_size_of_tag8
-  (x: U8.t)
-: Tot (y: U8.t { U8.v y == der_length_payload_size_of_tag x } )
-= [@inline_let]
-  let _ =
-    assert_norm (der_length_max == pow2 (8 * 126) - 1);
-    assert_norm (pow2 7 == 128);
-    assert_norm (pow2 8 == 256);
-    assert_norm (256 < der_length_max);
-    assert (U8.v x <= der_length_max)
-  in
-  if x `U8.lt` 129uy || x = 255uy
-  then
-    0uy
-  else
-    x `U8.sub` 128uy
-
-inline_for_extraction
-let log256_32
-  (n: U32.t { U32.v n > 0 } )
-: Tot (y: U8.t { U8.v y == log256' (U32.v n) } )
-= if n `U32.lt` 256ul
-  then 1uy
-  else if n `U32.lt` 65536ul
-  then 2uy
-  else if n `U32.lt` 16777216ul
-  then 3uy
-  else 4uy
-
-inline_for_extraction
-let tag_of_der_length32_impl
-  (x: U32.t)
-: Tot (y: U8.t { U32.v x < der_length_max /\ y == tag_of_der_length (U32.v x) } )
-= [@inline_let]
-  let _ = assert_norm (4294967296 <= der_length_max) in
-  if x `U32.lt` 128ul
-  then begin
-    [@inline_let] let _ = FStar.Math.Lemmas.small_modulo_lemma_1 (U32.v x) 256 in
-    Cast.uint32_to_uint8 x <: U8.t
-  end else
-    let len_len = log256_32 x in
-    [@inline_let] let _ =
-      log256_eq (U32.v x);
-      assert_norm (der_length_max == pow2 (8 * 126) - 1);
-      Math.pow2_lt_recip (8 * (U8.v len_len - 1)) (8 * 126)
-    in
-    128uy `U8.add` len_len
-
 #push-options "--max_ifuel 2"
 
 let parse32_bounded_der_length32
